---
title: "Assignment 2"
author: "Jakub Domasik"
date: "5 11 2019"
output: html_document
---

```{r setup, include=FALSE}
knitr::opts_chunk$set(echo = TRUE)
```

# Q1
### (a)

We want to find stationary point of:

$$f(u_{1:K}) = \sum_{i = 1}^{n} \sum_{k = 1}^{K} (\gamma_{ik} log( \prod_{j=1}^{n} u_{kj}^{x_{ij}}(1 - u_{kj})^{1 - x_{ij}}))$$

First, we expand the function:

$$f(u_{1:K}) = \sum_{i = 1}^{n} \sum_{i = 1}^{n} (\gamma_{ik} log( \prod_{j=1}^{n} \mu_{kj}^{x_{ij}}(1 - \mu_{kj})^{1 - x_{ij}})) = \sum_{i = 1}^{n} \sum_{i = 1}^{n} (\gamma_{ik} \sum_{j=1}^{P}(log(u_{kj}^{x_{ij}}(1-u_{kj})^{1-x_{ij}}))
=  \sum_{i = 1}^{n} \sum_{i = 1}^{n} (\gamma_{ik} \sum_{j=1}^{P}(x_{ij} log u_{kj} + (1-x_{ij}log(1-u_{kj})))$$

Next, we differentiate $f(u_{k})$ and set it equal to $0$:

$$f(u_{k})' =  \sum_{i = 1}^{n} \sum_{k = 1}^{K} (\gamma_{ik} \sum_{j=1}^{P}(\frac{x_{ij}}{u_{kj}} - \frac{1-x_{ij}}{1-u_{kj}})) = 0$$

The sum is qeual to 0, if for every k we have: 

 $$\sum_{i = 1}^{n} (\gamma_{ik} \sum_{j=1}^{P}(\frac{x_{ij}}{u_{kj}} - \frac{1-x_{ij}}{1-u_{kj}})) = 0$$
 
 Now, $\frac{x_{ij}}{u_{kj}} - \frac{1-x_{ij}}{1-u_{kj}}$
 are the entries of $\frac{x_{i}}{u_{k}} - \frac{1-x_{i}}{1-u_{k}}$  and  $x_{ij} \in {0,1}$ so:
 
 $$f(u_{k})' =  \sum_{i = 1}^{n} \sum_{k = 1}^{K} (\gamma_{ik} \sum_{j=1}^{P}(\frac{x_{ij}}{u_{kj}} - \frac{1-x_{ij}}{1-u_{kj}})) = 0 \iff \sum_{i=1}^{n}(\gamma_{ik} \sum_{j=1}^{P}(\frac{x_{i}}{u_{k}} - \frac{1-x_{i}}{1-u_{k}})) = 0$$
 Next, 
 $$ \sum_{i=1}^{n}(\gamma_{ik} \sum_{j=1}^{P}(\frac{x_{i}}{u_{k}} - \frac{1-x_{i}}{1-u_{k}})) = 
 \sum_{i=1}^{n} \gamma_{ik} \frac{x_{i}}{u_{k}} - \sum_{i=1}^{n} \gamma_{ik} \frac{1-x_{i}}{1-u_{k}}=0$$
 So,
 $$ \sum_{i=1}^{n} \gamma_{ik} \frac{x_{i}}{u_{k}} = \sum_{i=1}^{n} \gamma_{ik} \frac{1-x_{i}}{1-u_{k}}=0 \iff \\ u_{k} \sum_{i=1}^{n} \gamma_{ik}(1-x_{i}) = (1-u_{k}) \sum_{i=1}^{n} \gamma_{ik} x_{i} \iff \\
 u_{k}(\sum_{i=1}^{n} \gamma_{ik} x_{i} + \sum_{i=1}^{n} \gamma_{ik} (1-x_{i})) = \sum_{i=1}^{n} \gamma_{ik} x_{i} \iff \\ u_{k} = \frac{ \sum_{i=1}^{n} \gamma_{ik} x_{i}}{(\sum_{i=1}^{n} \gamma_{ik} x_{i} + \sum_{i=1}^{n} \gamma_{ik} (1-x_{i}))} = \frac{\sum_{i=1}^{n} \gamma_{ik}x_{i}}{\sum_{i=1}^{n}\gamma_{ik}}$$
 